{
 "cells": [
  {
   "cell_type": "markdown",
   "metadata": {},
   "source": [
    "# Functional Programming SS19\n",
    "\n",
    "# Assignment 07 Solutions"
   ]
  },
  {
   "cell_type": "markdown",
   "metadata": {},
   "source": [
    "### Exercise 1 (Transformation to Simple Haskell)\n",
    "\n",
    "*The data structure `List a` is defined by*\n",
    "\n",
    "```\n",
    "data List a = Nil | Cons a (List a)\n",
    "```\n",
    "\n",
    "*Transform the following Haskell-expression to an equivalent simple Haskell-expression using the transformation rules (1)-(9) from the lecture. Please give all intermediate expressions and indicate in each step which transformation rule was used. You may apply rules to several identical subterms simultaneously.*\n",
    "\n",
    "```\n",
    "let length Nil = 0\n",
    "    length (Cons x xs) = 1 + length xs\n",
    "in length xs\n",
    "```\n",
    "\n",
    "*Please simplify the intermediate expressions according to the following rules:*\n",
    "\n",
    "(i) `if (isa`$_{nâˆ’tuple}$ `exp) then exp1 else exp2` should be replaced by `exp1` for any $n \\leq 0$\n",
    "\n",
    "(ii) `(\\var -> exp1) exp` should be replaced by `exp1'`, where `exp1'` results from `exp1` by replacing all (free) occurrences of var by `exp`."
   ]
  },
  {
   "cell_type": "markdown",
   "metadata": {},
   "source": [
    "```\n",
    "let length Nil = 0\n",
    "    length (Cons x xs) = 1 + length xs\n",
    "in length xs\n",
    "```\n",
    "\n",
    "$(1) \\implies$\n",
    "\n",
    "```\n",
    "let length = \\x1 -> case x1 of Nil -> 0\n",
    "                               (Cons x xs) -> 1 + length xs\n",
    "in length xs\n",
    "```\n",
    "\n",
    "$(4) \\implies$\n",
    "\n",
    "```\n",
    "let length = \\x1 -> match Nil x1 0\n",
    "                    (match (Cons x xs) (1 + length xs) bot)\n",
    "in length xs\n",
    "```\n",
    "\n",
    "$(7) \\implies$\n",
    "\n",
    "```\n",
    "let length = \\x1 ->\n",
    "               if (isa_{Nil} x1)\n",
    "               then (match () (argof_{Nil} x1) 0\n",
    "                           (if (isa_{Cons} x1)\n",
    "                            then match (x, xs)\n",
    "                                       (argof_{Cons} x1)\n",
    "                                       (1 + length xs)\n",
    "                                       bot)\n",
    "                            else bot))\n",
    "               else (if (isa_{Cons} x1)\n",
    "                     then (match (x, xs)\n",
    "                                 (argof_{Cons} x1)\n",
    "                                 (1 + length xs)\n",
    "                                 bot)\n",
    "                     else bot)\n",
    "in length xs\n",
    "```\n",
    "\n",
    "$(8) \\implies$\n",
    "\n",
    "```\n",
    "let length = \\x1 ->\n",
    "               if (isa_{Nil} x1)\n",
    "               then (if (isa_{0-tuple} (argof_{Nil} x1))\n",
    "                     then 0\n",
    "                     else (if (isa_{Cons} x1)\n",
    "                            then match (x, xs)\n",
    "                                       (argof_{Cons} x1)\n",
    "                                       (1 + length xs)\n",
    "                                       bot)\n",
    "                            else bot))\n",
    "               else (if (isa_{Cons} x1)\n",
    "                     then (match (x, xs)\n",
    "                                 (argof_{Cons} x1)\n",
    "                                 (1 + length xs)\n",
    "                                 bot)\n",
    "                     else bot)\n",
    "in length xs\n",
    "```\n",
    "\n",
    "$(9) \\implies$\n",
    "\n",
    "```\n",
    "let length = \\x1 ->\n",
    "               if (isa_{Nil} x1)\n",
    "               then (if (isa_{0-tuple} (argof_{Nil} x1))\n",
    "                     then 0\n",
    "                     else (if (isa_{Cons} x1)\n",
    "                            then (if (isa_{2-tuple} (argof_{Cons} x1))\n",
    "                                  then match x (sel_{2,1} (argof_{Cons} x1))\n",
    "                                       (match xs (sel_{2,2} (argof_{Cons} x1))\n",
    "                                           (1 + length xs)\n",
    "                                           bot))\n",
    "                            else bot))\n",
    "               else (if (isa_{Cons} x1)\n",
    "                     then (if (isa_{2-tuple} (argof_{Cons} x1))\n",
    "                           then match x (sel_{2,1} (argof_{Cons} x1))\n",
    "                                (match xs (sel_{2,2} (argof_{Cons} x1))\n",
    "                                     (1 + length xs)\n",
    "                                     bot))\n",
    "                     else bot)\n",
    "in length xs\n",
    "```\n",
    "\n",
    "Since we know that `isa_{0-tuple} (argof_{Nil} x1)` is indeed the case based on the given definition of `List`, we can replace this expression by `0`. Similarly, we know that `isa_{2-tuple} (argof_{Cons} x1)` is also the case. We thus have\n",
    "\n",
    "```\n",
    "let length = \\x1 ->\n",
    "               if (isa_{Nil} x1)\n",
    "               then 0\n",
    "               else (if (isa_{Cons} x1)\n",
    "                     then match x (sel_{2,1} (argof_{Cons} x1))\n",
    "                          (match xs (sel_{2,2} (argof_{Cons} x1))\n",
    "                               (1 + length xs)\n",
    "                               bot)\n",
    "                     else bot)\n",
    "in length xs\n",
    "```\n",
    "\n",
    "$(7) \\implies$\n",
    "\n",
    "```\n",
    "let length = \\x1 ->\n",
    "               if (isa_{Nil} x1)\n",
    "               then 0\n",
    "               else (if (isa_{Cons} x1)\n",
    "                     then (\\x -> (\\xs -> (1 + length xs))\n",
    "                                     (sel_{2,2} (argof_{Cons} x1)))\n",
    "                              (sel_{2,1} (argof_{Cons} x1)))\n",
    "in length xs\n",
    "```\n",
    "\n",
    "We can now apply the second hint two successive times. After the first application to the innermost lambda, we have:\n",
    "\n",
    "```\n",
    "let length = \\x1 ->\n",
    "               if (isa_{Nil} x1)\n",
    "               then 0\n",
    "               else (if (isa_{Cons} x1)\n",
    "                     then (\\x -> (1 + length (sel_{2,2} (argof_{Cons} x1))))\n",
    "                              (sel_{2,1} (argof_{Cons} x1)))\n",
    "in length xs\n",
    "```\n",
    "\n",
    "After the second application, we obtain:\n",
    "\n",
    "```\n",
    "let length = \\x1 ->\n",
    "               if (isa_{Nil} x1)\n",
    "               then 0\n",
    "               else (if (isa_{Cons} x1)\n",
    "                     then (1 + length (sel_{2,2} (argof_{Cons} x1))))\n",
    "in length xs\n",
    "```\n",
    "\n",
    "None of the reduction rules are applicable anymore, so this is our resulting simple Haskell expression."
   ]
  },
  {
   "cell_type": "markdown",
   "metadata": {},
   "source": [
    "### Exercise 2 (Substitutions)\n",
    "\n",
    "*Identify the free variables of the following lambda terms $t_1$, $t_2$, and $t_3$, and also apply the three substitutions $\\sigma_1 = [x/\\lambda x.x \\; y]$, $\\sigma_2 = [y/v \\; y]$, and $\\sigma_3 = [z / \\lambda z.x \\; z]$ respectively, to each of these terms (so that you obtain in total 9 possibly different lambda terms $t_i\\sigma_j$ with $i, j \\in \\{ 1, 2, 3 \\}$):*\n",
    "\n",
    "a) $t_1 = \\lambda y.x \\; (\\lambda x.y \\; x)$\n",
    "\n",
    "b) $t_2 = \\lambda x.(\\lambda y.x \\; y) \\; x \\; y$\n",
    "\n",
    "c) $t_3 = \\lambda y.(\\lambda z.z \\; x \\; y) \\; z \\; y$"
   ]
  },
  {
   "cell_type": "markdown",
   "metadata": {},
   "source": [
    "Before we start with the identification of the free variables of $t_1$, $t_2$, and $t_3$ and the substitutions, let us identify the free variables of the terms that will be substituted.\n",
    "\n",
    "\\begin{align*}\n",
    "    \\operatorname{free}(\\lambda x.x \\; y) &= \\operatorname{free}(x \\; y) \\setminus \\{ x \\} \\\\\n",
    "    &= (\\operatorname{free}(x) \\cup \\operatorname{free}(y)) \\setminus \\{ x \\} \\\\\n",
    "    &= (\\{ x \\} \\cup \\{ y \\}) \\setminus \\{ x \\} \\\\\n",
    "    &= \\{ x, y \\} \\setminus \\{ x \\} \\\\\n",
    "    &= \\{ y \\} \\\\~\\\\\n",
    "    \\operatorname{free}(v \\; y) &= \\operatorname{free}(v) \\cup \\operatorname{free}(y) \\\\\n",
    "    &= \\{ v \\} \\cup \\{ y \\} \\\\\n",
    "    &= \\{ v, y \\} \\\\~\\\\\n",
    "    \\operatorname{free}(\\lambda z.x \\; z) &= \\operatorname{free}(x \\; z) \\setminus \\{ z \\} \\\\\n",
    "    &= (\\operatorname{free}(x) \\cup \\operatorname{free}(z)) \\setminus \\{ z \\} \\\\\n",
    "    &= (\\{ x \\} \\cup \\{ z \\}) \\setminus \\{ z \\} \\\\\n",
    "    &= \\{ x, z \\} \\setminus \\{ z \\} \\\\\n",
    "    &= \\{ x \\}\n",
    "\\end{align*}"
   ]
  },
  {
   "cell_type": "markdown",
   "metadata": {},
   "source": [
    "a) $t_1 = \\lambda y.x \\; (\\lambda x.y \\; x)$\n",
    "\n",
    "\\begin{align*}\n",
    "    \\operatorname{free}(\\lambda y.x \\; (\\lambda x.y \\; x)) &= \\operatorname{free}(x \\; (\\lambda x.y \\; x)) \\setminus \\{ y \\} \\\\\n",
    "    &= (\\operatorname{free}(x) \\cup \\operatorname{free}(\\lambda x.y \\; x)) \\setminus \\{ y \\} \\\\\n",
    "    &= (\\{ x \\} \\cup \\operatorname{free}(\\lambda x.(y \\; x))) \\setminus \\{ y \\} \\\\\n",
    "    &= (\\{ x \\} \\cup \\operatorname{free}(y \\; x) \\setminus \\{ x \\}) \\setminus \\{ y \\} \\\\\n",
    "    &= (\\{ x \\} \\cup (\\operatorname{free}(y) \\cup \\operatorname{free}(x)) \\setminus \\{ x \\}) \\setminus \\{ y \\} \\\\\n",
    "    &= (\\{ x \\} \\cup (\\{ y \\} \\cup \\{ x \\}) \\setminus \\{ x \\}) \\setminus \\{ y \\} \\\\\n",
    "    &= (\\{ x \\} \\cup \\{ x, y \\} \\setminus \\{ x \\}) \\setminus \\{ y \\} \\\\\n",
    "    &= (\\{ x, y \\} \\setminus \\{ x \\}) \\setminus \\{ y \\} \\\\\n",
    "    &= \\{ y \\} \\setminus \\{ y \\} \\\\\n",
    "    &= \\varnothing\n",
    "\\end{align*}"
   ]
  },
  {
   "cell_type": "markdown",
   "metadata": {},
   "source": [
    "Applying the substitution rules in definition 3.1.3, we have:\n",
    "\n",
    "\\begin{align*}\n",
    "    t_1\\sigma_1 &= (\\lambda y.x \\; (\\lambda x.y \\; x))[x/\\lambda x.x \\; y] \\\\\n",
    "    &= \\lambda y'.((x \\; (\\lambda x.y \\; x))[y/y'][x/\\lambda x.x \\; y]) \\\\\n",
    "    &= \\lambda y'.((x)[y/y'][x/\\lambda x.x \\; y] \\; (\\lambda x.y \\; x)[y/y'][x/\\lambda x.x \\; y]) \\\\\n",
    "    &= \\lambda y'.(\\lambda x.x \\; y) \\; (\\lambda x.y' \\; x) \\\\~\\\\\n",
    "    t_1\\sigma_2 &= (\\lambda y.x \\; (\\lambda x.y \\; x))[y/v \\; y] \\\\\n",
    "    &= \\lambda y.x \\; (\\lambda x.y \\; x) \\\\~\\\\\n",
    "    t_1\\sigma_3 &= (\\lambda y.x \\; (\\lambda x.y \\; x))[z / \\lambda z.x \\; z] \\\\\n",
    "    &= \\lambda y.((x \\; (\\lambda x.y \\; x))[z / \\lambda z.x \\; z]) \\\\\n",
    "    &= \\lambda y.((x)[z / \\lambda z.x \\; z] \\; (\\lambda x.y \\; x)[z / \\lambda z.x \\; z]) \\\\\n",
    "    &= \\lambda y.x \\; (\\lambda x.y \\; x)\n",
    "\\end{align*}"
   ]
  },
  {
   "cell_type": "markdown",
   "metadata": {},
   "source": [
    "b) $t_2 = \\lambda x.(\\lambda y.x \\; y) \\; x \\; y$"
   ]
  },
  {
   "cell_type": "markdown",
   "metadata": {},
   "source": [
    "\\begin{align*}\n",
    "    \\operatorname{free}(\\lambda x.(\\lambda y.x \\; y) \\; x \\; y) &= \\operatorname{free}(\\lambda x.((\\lambda y.x \\; y) \\; x) \\; y) \\\\\n",
    "    &= \\operatorname{free}(((\\lambda y.x \\; y) \\; x) \\; y) \\setminus \\{ x \\} \\\\\n",
    "    &= (\\operatorname{free}((\\lambda y.x \\; y) \\; x) \\cup \\operatorname{free}(y)) \\setminus \\{ x \\} \\\\\n",
    "    &= (\\operatorname{free}((\\lambda y.x \\; y) \\; x) \\cup \\{ y \\}) \\setminus \\{ x \\} \\\\\n",
    "    &= ((\\operatorname{free}(\\lambda y.x \\; y) \\cup \\operatorname{free}(x)) \\cup \\{ y \\}) \\setminus \\{ x \\} \\\\\n",
    "    &= (((\\operatorname{free}(x \\; y) \\setminus \\{ y \\}) \\cup \\{ x \\}) \\cup \\{ y \\}) \\setminus \\{ x \\} \\\\\n",
    "    &= ((((\\operatorname{free}(x) \\cup \\operatorname{free}(y)) \\setminus \\{ y \\}) \\cup \\{ x \\}) \\cup \\{ y \\}) \\setminus \\{ x \\} \\\\\n",
    "    &= ((((\\{ x \\} \\cup \\{ y \\}) \\setminus \\{ y \\}) \\cup \\{ x \\}) \\cup \\{ y \\}) \\setminus \\{ x \\} \\\\\n",
    "    &= (((\\{ x, y \\} \\setminus \\{ y \\}) \\cup \\{ x \\}) \\cup \\{ y \\}) \\setminus \\{ x \\} \\\\\n",
    "    &= ((\\{ x \\} \\cup \\{ x \\}) \\cup \\{ y \\}) \\setminus \\{ x \\} \\\\\n",
    "    &= (\\{ x \\} \\cup \\{ y \\}) \\setminus \\{ x \\} \\\\\n",
    "    &= \\{ x, y \\} \\setminus \\{ x \\} \\\\\n",
    "    &= \\{ y \\}\n",
    "\\end{align*}"
   ]
  },
  {
   "cell_type": "markdown",
   "metadata": {},
   "source": [
    "For the substitutions, we have:\n",
    "\n",
    "\\begin{align*}\n",
    "    t_2\\sigma_1 &= (\\lambda x.(\\lambda y.x \\; y) \\; x \\; y)[x/\\lambda x.x \\; y] \\\\\n",
    "    &= \\lambda x.(\\lambda y.x \\; y) \\; x \\; y \\\\~\\\\\n",
    "    t_2\\sigma_2 &= (\\lambda x.(\\lambda y.x \\; y) \\; x \\; y)[y/v \\; y] \\\\\n",
    "    &= \\lambda x.(((\\lambda y.x \\; y) \\; x \\; y)[y/v \\; y]) \\\\\n",
    "    &= \\lambda x.((((\\lambda y.x \\; y) \\; x) \\; y)[y/v \\; y]) \\\\\n",
    "    &= \\lambda x.(((\\lambda y.x \\; y) \\; x)[y/v \\; y] \\; (y)[y/v \\; y]) \\\\\n",
    "    &= \\lambda x.(((\\lambda y.x \\; y)[y/v \\; y] \\; (x)[y/v \\; y]) \\; v \\; y) \\\\\n",
    "    &= \\lambda x.((\\lambda y.x \\; y) \\; x) \\; v \\; y \\\\\n",
    "    &= \\lambda x.(\\lambda y.x \\; y) \\; x \\; v \\; y \\\\~\\\\\n",
    "    t_2\\sigma_3 &= (\\lambda x.(\\lambda y.x \\; y) \\; x \\; y)[z / \\lambda z.x \\; z] \\\\\n",
    "    &= \\lambda x.(((\\lambda y.x \\; y) \\; x \\; y)[z / \\lambda z.x \\; z]) \\\\\n",
    "    &= \\lambda x.((((\\lambda y.x \\; y) \\; x) \\; y)[z / \\lambda z.x \\; z]) \\\\\n",
    "    &= \\lambda x.(((\\lambda y.x \\; y) \\; x)[z / \\lambda z.x \\; z] \\; (y)[z / \\lambda z.x \\; z]) \\\\\n",
    "    &= \\lambda x.(((\\lambda y.x \\; y)[z / \\lambda z.x \\; z] \\; (x)[z / \\lambda z.x \\; z]) \\; y) \\\\\n",
    "    &= \\lambda x.(((\\lambda y.((x \\; y)[z / \\lambda z.x \\; z])) \\; x) \\; y) \\\\\n",
    "    &= \\lambda x.((\\lambda y.((x)[z / \\lambda z.x \\; z] \\; (y)[z / \\lambda z.x \\; z]) \\; x) \\; y) \\\\\n",
    "    &= \\lambda x.(((\\lambda y.(x \\; y)) \\; x) \\; y) \\\\\n",
    "    &= \\lambda x.((\\lambda y.(x \\; y)) \\; x) \\; y \\\\\n",
    "    &= \\lambda x.(\\lambda y.(x \\; y)) \\; x \\; y \\\\\n",
    "    &= \\lambda x.(\\lambda y.x \\; y) \\; x \\; y \\\\\n",
    "\\end{align*}"
   ]
  },
  {
   "cell_type": "markdown",
   "metadata": {},
   "source": [
    "c) $t_3 = \\lambda y.(\\lambda z.z \\; x \\; y) \\; z \\; y$"
   ]
  },
  {
   "cell_type": "markdown",
   "metadata": {},
   "source": [
    "\\begin{align*}\n",
    "    \\operatorname{free}(\\lambda y.(\\lambda z.z \\; x \\; y) \\; z \\; y) &= \\operatorname{free}(\\lambda y.((\\lambda z.z \\; x \\; y) \\; z) \\; y) \\\\\n",
    "    &= \\operatorname{free}((\\lambda z.(z \\; x \\; y) \\; z) \\; y) \\setminus \\{ y \\} \\\\\n",
    "    &= \\operatorname{free}(((\\lambda z.(z \\; x) \\; y) \\; z) \\; y) \\setminus \\{ y \\} \\\\\n",
    "    &= (\\operatorname{free}((\\lambda z.(z \\; x) \\; y) \\; z) \\cup \\operatorname{free}(y)) \\setminus \\{ y \\} \\\\\n",
    "    &= ((\\operatorname{free}(\\lambda z.(z \\; x) \\; y) \\cup \\operatorname{free}(z)) \\cup \\{ y \\}) \\setminus \\{ y \\} \\\\\n",
    "    &= (((\\operatorname{free}((z \\; x) \\; y) \\setminus \\{ z \\}) \\cup \\{ z \\}) \\cup \\{ y \\}) \\setminus \\{ y \\} \\\\\n",
    "    &= ((((\\operatorname{free}(z \\; x) \\cup \\operatorname{free}(y)) \\setminus \\{ z \\}) \\cup \\{ z \\}) \\cup \\{ y \\}) \\setminus \\{ y \\} \\\\\n",
    "    &= (((((\\operatorname{free}(z) \\cup \\operatorname{free}(x)) \\cup \\{ y \\}) \\setminus \\{ z \\}) \\cup \\{ z \\}) \\cup \\{ y \\}) \\setminus \\{ y \\} \\\\\n",
    "    &= (((((\\{ z \\} \\cup \\{ x \\}) \\cup \\{ y \\}) \\setminus \\{ z \\}) \\cup \\{ z \\}) \\cup \\{ y \\}) \\setminus \\{ y \\} \\\\\n",
    "    &= ((((\\{ x, z \\} \\cup \\{ y \\}) \\setminus \\{ z \\}) \\cup \\{ z \\}) \\cup \\{ y \\}) \\setminus \\{ y \\} \\\\\n",
    "    &= (((\\{ x, y, z \\} \\setminus \\{ z \\}) \\cup \\{ z \\}) \\cup \\{ y \\}) \\setminus \\{ y \\} \\\\\n",
    "    &= ((\\{ x, y \\} \\cup \\{ z \\}) \\cup \\{ y \\}) \\setminus \\{ y \\} \\\\\n",
    "    &= (\\{ x, y, z \\} \\cup \\{ y \\}) \\setminus \\{ y \\} \\\\\n",
    "    &= \\{ x, y, z \\} \\setminus \\{ y \\} \\\\\n",
    "    &= \\{ x, z \\}\n",
    "\\end{align*}"
   ]
  },
  {
   "cell_type": "markdown",
   "metadata": {},
   "source": [
    "The substitutions are given as follows:\n",
    "\n",
    "\\begin{align*}\n",
    "    t_3\\sigma_1 &= (\\lambda y.(\\lambda z.z \\; x \\; y) \\; z \\; y)[x/\\lambda x.x \\; y] \\\\\n",
    "    &= \\lambda y'.(((\\lambda z.z \\; x \\; y') \\; z \\; y')[x/\\lambda x.x \\; y]) \\\\\n",
    "    &= \\lambda y'.((((\\lambda z.z \\; x \\; y') \\; z) \\; y')[x/\\lambda x.x \\; y]) \\\\\n",
    "    &= \\lambda y'.(((\\lambda z.z \\; x \\; y') \\; z)[x/\\lambda x.x \\; y] \\; (y')[x/\\lambda x.x \\; y]) \\\\\n",
    "    &= \\lambda y'.(((\\lambda z.z \\; x \\; y')[x/\\lambda x.x \\; y] \\; (z)[x/\\lambda x.x \\; y]) \\; y') \\\\\n",
    "    &= \\lambda y'.((\\lambda z.(z \\; x \\; y')[x/\\lambda x.x \\; y] \\; z) \\; y') \\\\\n",
    "    &= \\lambda y'.((\\lambda z.((z \\; x) \\; y')[x/\\lambda x.x \\; y] \\; z) \\; y') \\\\\n",
    "    &= \\lambda y'.((\\lambda z.((z \\; x)[x/\\lambda x.x \\; y] \\; (y')[x/\\lambda x.x \\; y]) \\; z) \\; y') \\\\\n",
    "    &= \\lambda y'.((\\lambda z.(((z)[x/\\lambda x.x \\; y] \\; (x)[x/\\lambda x.x \\; y]) \\; y') \\; z) \\; y') \\\\\n",
    "    &= \\lambda y'.((\\lambda z.((z \\; (\\lambda x.x \\; y)) \\; y') \\; z) \\; y') \\\\\n",
    "    &= \\lambda y'.((\\lambda z.(z \\; (\\lambda x.x \\; y) \\; y') \\; z) \\; y') \\\\\n",
    "    &= \\lambda y'.(\\lambda z.(z \\; (\\lambda x.x \\; y) \\; y') \\; z) \\; y' \\\\\n",
    "    &= (\\lambda y'.(\\lambda z.z \\; (\\lambda x.x \\; y) \\; y') \\; z) \\; y' \\\\\n",
    "    &= \\lambda y'.(\\lambda z.z \\; (\\lambda x.x \\; y) \\; y') \\; z \\; y' \\\\~\\\\\n",
    "    t_3\\sigma_2 &= (\\lambda y.(\\lambda z.z \\; x \\; y) \\; z \\; y)[y/v \\; y] \\\\\n",
    "    &= \\lambda y.(\\lambda z.z \\; x \\; y) \\; z \\; y \\\\~\\\\\n",
    "    t_3\\sigma_3 &= (\\lambda y.(\\lambda z.z \\; x \\; y) \\; z \\; y)[z / \\lambda z.x \\; z] \\\\\n",
    "    &= \\lambda y.(((\\lambda z.z \\; x \\; y) \\; z \\; y)[z / \\lambda z.x \\; z]) \\\\\n",
    "    &= \\lambda y.((((\\lambda z.z \\; x \\; y) \\; z) \\; y)[z / \\lambda z.x \\; z]) \\\\\n",
    "    &= \\lambda y.(((\\lambda z.z \\; x \\; y) \\; z)[z / \\lambda z.x \\; z] \\; (y)[z / \\lambda z.x \\; z]) \\\\\n",
    "    &= \\lambda y.(((\\lambda z.z \\; x \\; y)[z / \\lambda z.x \\; z] \\; (z)[z / \\lambda z.x \\; z]) \\; y) \\\\\n",
    "    &= \\lambda y.(((\\lambda z.z \\; x \\; y) \\; (\\lambda z.x \\; z)) \\; y) \\\\\n",
    "    &= \\lambda y.((\\lambda z.z \\; x \\; y) \\; (\\lambda z.x \\; z) \\; y) \\\\\n",
    "    &= \\lambda y.(\\lambda z.z \\; x \\; y) \\; (\\lambda z.x \\; z) \\; y\n",
    "\\end{align*}"
   ]
  },
  {
   "cell_type": "markdown",
   "metadata": {},
   "source": [
    "### Exercise 3 ($\\beta$-reduction)\n",
    "\n",
    "a) *Give all reduction sequences with $\\rightarrow_{\\beta}$ starting with the following term:*\n",
    "\n",
    "\\begin{equation*}\n",
    "    (\\lambda x \\; y.x \\; y) \\text{ exp } ((\\lambda x \\; z. \\text{mult } x \\; (\\text{mult } z \\; z)) \\; 3 \\; 2)\n",
    "\\end{equation*}\n",
    "\n",
    "b) *Give all reduction sequences $\\rightarrow_{\\beta}$ with at most 3 steps starting with the following term:*\n",
    "\n",
    "\\begin{equation*}\n",
    "    (\\lambda f.(\\lambda x. \\; f \\; (x \\; x)) \\; (\\lambda x. \\; f \\; (x \\; x))) \\; (\\lambda y.y)\n",
    "\\end{equation*}\n",
    "\n",
    "***Hints:***\n",
    "\n",
    "* *You can save space by representing the reduction sequences as directed graphs. For example, $t_1 \\rightarrow_{\\beta} t_2 \\rightarrow_{\\beta} t_4$, $t_1 \\rightarrow_{\\beta} t_2 \\rightarrow_{\\beta} t_5$, and $t_1 \\rightarrow_{\\beta} t_3 \\rightarrow_{\\beta} t_5$ can be represented as:*\n",
    "\n",
    "![reduction_sequence_graph](reduction_sequence_graph.png)\n",
    "\n",
    "* *In a), you may abbreviate `exp` to `e` and `mult` to `m` to save space.*\n",
    "* *In b), you may write $A_f$ instead of $\\lambda x.f \\; (x \\; x)$, $B$ instead of $\\lambda y.y$ and $C$ instead of $\\lambda x.x \\; x$ to save space. The start term could then be represented as $(\\lambda f.A_f \\; A_f) \\; B$. Furthermore, the term $\\lambda x.(\\lambda y.y) \\; (x \\; x)$ can be abbreviated to $A_B$.*"
   ]
  },
  {
   "cell_type": "markdown",
   "metadata": {},
   "source": [
    "a) The graph showing the $\\rightarrow_\\beta$ reduction sequences for $(\\lambda x \\; y.x \\; y) \\text{ exp } ((\\lambda x \\; z. \\text{mult } x \\; (\\text{mult } z \\; z)) \\; 3 \\; 2)$ is given below.\n",
    "\n",
    "![3a_beta_reduction_sequences](3a_beta_reduction_sequences.png)"
   ]
  },
  {
   "cell_type": "markdown",
   "metadata": {},
   "source": [
    "b) The $\\rightarrow_{\\beta}$ reduction sequences for $(\\lambda f.(\\lambda x. \\; f \\; (x \\; x)) \\; (\\lambda x. \\; f \\; (x \\; x))) \\; (\\lambda y.y)$ with at most three steps are shown in the graph below.\n",
    "\n",
    "![3b_beta_reduction_sequences](3b_beta_reduction_sequences.png)"
   ]
  },
  {
   "cell_type": "markdown",
   "metadata": {},
   "source": [
    "### Exercise 4 (Confluence)\n",
    "\n",
    "a) *Let $\\mathbb{N} = \\{ 0, 1, 2, ... \\}$ be the natural numbers with the standard relation $>$. Indicate whether the following properties hold. Explain your solution!*\n",
    "\n",
    "* *For any $n \\in \\mathbb{N}$ there is an $m \\in \\mathbb{N}$ such that $m$ is a normal form of $n$ w.r.t. $>$.*\n",
    "* *$>$ is confluent.*"
   ]
  },
  {
   "cell_type": "markdown",
   "metadata": {},
   "source": [
    "Based on definition 3.2.3, the transitive-reflexive closure of $>$ is the relation $\\geq$ since for any $t_1, t_2, t_3 \\in \\mathbb{N}$, it holds that\n",
    "* $t_1 > t_2 \\implies t_1 \\geq t_2$\n",
    "* $t_1 > t_2 \\geq t_3 \\implies t_1 \\geq t_3$\n",
    "* $t_1 \\geq t_1$\n",
    "\n",
    "---\n",
    "\n",
    "According to the same definition, a number $m \\in \\mathbb{N}$ is a normal form of $n \\in \\mathbb{N}$ w.r.t $>$ iff $n \\geq m$ and $m$ is a normal form, which is the case iff there is no $q \\in \\mathbb{N}$ for which $m > q$. The normal form of $\\mathbb{N}$ is $m = 0$ since there is no $q \\in \\mathbb{N}$ such that $m > q$. Since it also holds that $n \\geq 0$ for any $n \\in \\mathbb{N}$, we see that the first property holds. $\\square$\n",
    "\n",
    "---\n",
    "\n",
    "$>$ is confluent if for every $t, q_1, q_2 \\in \\mathbb{N}$ we have that, whenever $t \\geq q_1$ and $t \\geq q_2$, there is a $q \\in \\mathbb{N}$ such that $g_1 \\geq q$ and $g_2 \\geq q$. Let us investigate four exhaustive cases to show that the confluence property holds:\n",
    "\n",
    "1. If $t = q_1 = q_2$, the property clearly holds since we can then take $q = t$ to satisfy it.\n",
    "\n",
    "2. Without loss of generality, if we assume $t = q_1 \\neq q_2$, we can take $q = q_2$ to satisfy it since $q_1 = t \\geq q$ and $q_2 = q \\geq q$.\n",
    "\n",
    "3. If $q_1 = q_2 \\neq t$, we can, without loss of generality, take $q = q_1$ to satisfy the property since $q_1 = q \\geq q$ and $q_2 = q \\geq q$.\n",
    "\n",
    "4. In the most general case, $t \\neq q_1 \\neq q_2$. Since we know that $>$ has a normal form for any $n \\in \\mathbb{N}$, we can satisfy the property by taking $q = 0$ since $q_1 \\geq 0$ and $q_2 \\geq 0$.\n",
    "\n",
    "This proves that $>$ is confluent. $\\square$"
   ]
  },
  {
   "cell_type": "markdown",
   "metadata": {},
   "source": [
    "b) *Let $\\mathbb{N} = \\{ 0, 1, 2, ... \\}$ be the natural numbers with the following relation $\\succ: m \\succ n$ if there is some $0 < r \\in \\mathbb{N}$ with $m = r \\cdot n$, i.e. $n$ divides $m$. Indicate whether the following properties hold. Explain your solution!*\n",
    "\n",
    "* *For any $n \\in \\mathbb{N}$ there is an $m \\in \\mathbb{N}$ such that $m$ is a normal form of $n$ w.r.t. $\\succ$.*\n",
    "* *$\\succ$ is confluent.*"
   ]
  },
  {
   "cell_type": "markdown",
   "metadata": {},
   "source": [
    "The relation $\\succ$ is its own transitive-reflexive closure since for any $t_1, t_2, t_3 \\in \\mathbb{N}$, we have:\n",
    "\n",
    "* $t_1 \\succ t_2 \\implies t_2 \\succ t_2$\n",
    "* $t_1 \\succ t_2 \\succ t_3 \\implies t_1 \\implies t_3$ (proof: if we write $t_1 = mt_2$ and $t_2 = nt_3$ for some $0 < m, n \\in \\mathbb{N}$, then $t_1 = mt_2 = m(nt_3) = kt_3$ where $k = mn$).\n",
    "* $t_1 \\succ t_1$ (this clearly holds for any $m > 0$ since any number is divisible by itself; for the given definition of $\\succ$, this also holds for $m = 0$ since we can then take any $0 < r \\in \\mathbb{N}$ to satisfy the definition)\n",
    "\n",
    "---\n",
    "\n",
    "$m \\in \\mathbb{N}$ is a normal form of $n \\in \\mathbb{N}$ w.r.t. $>$ iff $n \\succ m$ and $m$ is a normal form. $m$ will be a normal form iff a $q \\in \\mathbb{N}$ for which $m \\succ q$ does not exist; however, as we know from before, $\\succ$ is reflexive and so for any $m$, we can take $q = m$ to satisfy the relation. Thus, $m$ is not a normal form and can therefore not be a normal form of $n$. $\\square$\n",
    "\n",
    "---\n",
    "\n",
    "The relation $\\succ$ will be confluent if for any $t, q_1, q_2 \\in \\mathbb{N}$ such that $t \\succ q_1$ and $t \\succ q_2$, we can find a $q \\in \\mathbb{N}$ for which $q_1 \\succ q$ and $q_2 \\succ q$. This clearly holds since we can take $q = 1$ to satisfy the relation for any arbitrary $t, q_1, q_2$; thus, $\\succ$ is confluent. $\\square$"
   ]
  },
  {
   "cell_type": "markdown",
   "metadata": {},
   "source": [
    "c) *Let $\\mathbb{Z}$ be the integers with the standard relation $>$. Indicate whether the following properties hold. Explain your solution!*\n",
    "\n",
    "* *For any $z \\in \\mathbb{Z}$ there is a $q \\in \\mathbb{Z}$ such that $q$ is a normal form of $z$ w.r.t. $>$.*\n",
    "* *$>$ is confluent.*"
   ]
  },
  {
   "cell_type": "markdown",
   "metadata": {},
   "source": [
    "As in part a), the transitive-reflexive closure of $>$ will be the relation $\\geq$.\n",
    "\n",
    "---\n",
    "\n",
    "A number $q \\in \\mathbb{Z}$ is a normal form of $z \\in \\mathbb{Z}$ w.r.t. $>$ iff $z \\geq q$ and $q$ is a normal form. Now, $q$ is a normal form if there is no $q' \\in \\mathbb{Z}$ such that $q > q'$; however, for any $q$, we can always take $q' = q - 1 \\in \\mathbb{Z}$ so that $q > q'$. This means that $q$ cannot be a normal form and is thus not a normal form of $z$ w.r.t. $>$.\n",
    "\n",
    "---\n",
    "\n",
    "Let's proceed to show that $q$ is confluent as in part a), namely by considering $t, q_1, q_2 \\in \\mathbb{Z}$.\n",
    "\n",
    "1. The first three cases, namely $t = q_1 = q_2$, $t = q_1 \\neq q_2$, and $q1 = q_2 \\neq t$, can be treated the same as in a)\n",
    "2. For the most general case of $t \\neq q_1 \\neq q_2$, let us, without loss of generality, assume that $q_1 \\geq q_2$. Then, we can take $q = q_2 - 1$, in which case we have $q_1 \\geq q$ and $q_2 \\geq q$.\n",
    "\n",
    "Thus, $>$ is confluent. $\\square$"
   ]
  },
  {
   "cell_type": "markdown",
   "metadata": {},
   "source": [
    "d) *Let $\\operatorname{Pot}_{\\neq \\varnothing}(\\mathbb{Z})$ be the set of nonempty subsets of the integers with the relation $\\subsetneq: A \\subsetneq B$ whenever $A \\neq B$ and $A$ is a subset of $B$. Indicate whether the following properties hold. Explain your solution!*\n",
    "\n",
    "* *For any $\\varnothing \\neq A \\subseteq \\mathbb{Z}$ there is a $B \\subseteq \\mathbb{Z}$ such that $B$ is a normal form of $A$ w.r.t. $\\subsetneq$.*\n",
    "* *$\\subsetneq$ is confluent.*"
   ]
  },
  {
   "cell_type": "markdown",
   "metadata": {},
   "source": [
    "The transitive-reflexive closure of $\\subsetneq$ will be the relation $\\subseteq$ since for any $A, B, C \\subseteq \\mathbb{Z}$, we have:\n",
    "\n",
    "* $A \\subsetneq B \\implies A \\subseteq B$ \n",
    "* $A \\subsetneq B \\subseteq C \\implies A \\subseteq C$\n",
    "* $A \\subseteq A$\n",
    "\n",
    "---\n",
    "\n",
    "A set $\\varnothing \\neq B \\subseteq Z$ will be a normal form of $\\varnothing \\neq A \\subseteq Z$ iff $A \\subseteq B$ and $B$ is a normal form, which is the case if there is no $\\varnothing \\neq C \\subseteq Z$ such that $B \\subsetneq C$. The normal form of $\\mathbb{Z}$ is $B = \\mathbb{Z}$ since there is then no $C \\subseteq \\mathbb{Z}$ with $B \\subsetneq C$. Since every $A \\subseteq \\mathbb{Z} \\subseteq B = \\mathbb{Z}$, the first property holds. $\\square$\n",
    "\n",
    "---\n",
    "\n",
    "The relation $\\subsetneq$ is confluent if for any $A, B, C \\subseteq \\mathbb{Z}$, whenever $A \\subseteq B$ and $A \\subseteq C$, then there is a $Q \\subseteq \\mathbb{Z}$ such that $B \\subseteq Q$ and $C \\subseteq Q$. This clearly holds since we can take $Q = \\mathbb{Z}$, in which case $B \\subseteq Q$ and $C \\subseteq Q$. Thus, $\\subsetneq$ is confluent. $\\square$"
   ]
  }
 ],
 "metadata": {
  "kernelspec": {
   "display_name": "Haskell",
   "language": "haskell",
   "name": "haskell"
  },
  "language_info": {
   "codemirror_mode": "ihaskell",
   "file_extension": ".hs",
   "name": "haskell",
   "pygments_lexer": "Haskell",
   "version": "8.6.4"
  }
 },
 "nbformat": 4,
 "nbformat_minor": 2
}
